I made a number of changes to defunc and definec, some of which may have large consequences. One of the changes is that the output contract theorem are now forward chaining and rewrite rules, but not type prescription rules. I reduced the amount of exploration defunc does by better integrating any extra hints we get from users. I added force to each hypof function contracts for defunc. I added support for defuncb, where acl2s-bool-undefined is used for output contracts that state the function returns a boolean. All of this allowed me to unify the way defunc and definec work, so that led to simplifications to definec. Finally I added/fixed support for version of defunc, definec that disable the functions, don't test during function admissions, etc.

books/acl2s/definec.lisp
@@ -81,6 +81,8 @@ both expand into
 
 |#
 
+;; Before latest updates to defunc 
+
 (defmacro definec (name &rest args)
   `(with-output
     :stack :push :off :all
@@ -95,32 +97,11 @@ both expand into
           (f-type-pred (pred-of-type f-type tbl))
           (ic (make-input-contract d-args d-arg-preds))
           (oc (make-output-contract ',name d-args f-type-pred))
-          (fc-name (intern$ ,(concatenate 'acl2::string (symbol-name name) 
-                                          "-DEFINEC-FC-RULE")
-                            pkg))
-          (f-contract-name
-           (intern$ ,(concatenate 'acl2::string (symbol-name name)
-                                  "-CONTRACT")
-                    pkg))
           (defunc `(defunc ,',name ,d-args
                      :input-contract ,ic
                      :output-contract ,oc
-                     ,@(cddr ',args)))
-          (defthm (if (equal oc t)
-                      '(value-triple :passed)
-                    `(defthm ,fc-name (implies (force ,ic) ,oc)
-                       :hints (("goal"
-                                :instructions ((dv 1) r))
-                               ("goal'"
-                                :by ,f-contract-name))
-                       :rule-classes
-                       ((:forward-chaining
-                         :trigger-terms ((,',name ,@d-args))))))))
-         `(progn (with-output :stack :pop ,defunc)
-                 (with-output
-                  :off :all
-                  (make-event
-                   `(:or ,',defthm (value-triple :passed)))))))))
+                     ,@(cddr ',args))))
+         `(with-output :stack :pop ,defunc)))))
 
 #|
 
@@ -248,12 +229,17 @@ bells and whistles of @('acl2s::defunc').
   )
 
 (defmacro definecd (name &rest args)
-  (let* ((defname (make-symbl `(,name -DEFINITION-RULE))))
+  (let ((defname (make-symbl `(,name -DEFINITION-RULE))))
     `(progn
-      (definec ,name ,@args)
-      (in-theory (disable ,defname)))))
+       (definec ,name ,@args)
+       (in-theory (disable ,defname)))))
 
 (defmacro definec-no-test (name &rest args)
   `(acl2::with-outer-locals
     (local (acl2s-defaults :set testing-enabled nil))
     (definec ,name ,@args)))
+
+(defmacro definecd-no-test (name &rest args)
+  `(acl2::with-outer-locals
+    (local (acl2s-defaults :set testing-enabled nil))
+    (definecd ,name ,@args)))
